Dafny input clarification
Co-authored-by: Ben Manley <bdmanley@umich.edu>
Co-authored-by: jubeemer <jubeemer@users.noreply.github.com>

Test/591tests/lock_server.dfy
@@ -2,33 +2,75 @@
 // type server
 datatype Server = Server(id:int, semaphore:bool)
 datatype Client = Client(id:int, connServers:set<int>)
-datatype DafnyStateMachine = DafnyStateMachine(clients:set<Client>, servers:set<Server>)
+datatype DafnyState = DafnyState(clients:seq<Client>, servers:seq<Server>)
 
 // relation link(X:client, Y:server)
 // relation semaphore(X:server)
+predicate RelationLink(m: DafnyState, c: Client, s: Server)
+{
+    && 0 <= s.id < |m.servers|
+    && 0 <= c.id < |m.clients|
+    && m.servers[s.id].id in m.clients[c.id].connServers
+}
+
+predicate RelationSemaphore(m: DafnyState, s: Server)
+{
+    && 0 <= s.id < |m.servers|
+    && m.servers[s.id].semaphore
+}
 
 // after init {
 //     semaphore(W) := true;
 //     link(X,Y) := false
 // }
-predicate Init(m: DafnyStateMachine) {
-    (forall s:Server :: s in m.servers ==> s.semaphore == true)
-    && (forall c:Client :: c in m.clients ==> |c.connServers| == 0)
+predicate Init(m: DafnyState) {
+    && forall s: Server :: s in m.servers ==> RelationSemaphore(m, s)
+    && forall s: Server, c: Client :: s in m.servers && c in m.clients ==> !RelationLink(m, c, s)
 }
+
+// predicate ServerInit(s: Server, id: int) {
+//     s.semaphore == true && s.id == id
+// }
+
+// predicate ClientInit(c: Client, id: int) {
+//     |c.connServers| == 0  && c.id == id
+// }
+
+// predicate Connect(s: Server, s': Server, c: Client, c': Client) {
+//     && s.id == s'.id
+//     && c.id == c'.id
+//     && s.semaphore == true
+//     && s'.semaphore == false
+//     && s.id in c'.connServers
+// }
 
 // action connect(x:client,y:server) = {
 //   require semaphore(y);
 //   link(x,y) := true;
 //   semaphore(y) := false
 // }
-predicate Connect(m: DafnyStateMachine, m': DafnyStateMachine, c: Client, s: Server) {
-    && c in m.clients // client exists
-    && s in m.servers // server exists
-    && s.semaphore == true // server is unlocked to start
-    && Client(c.id, c.connServers + {s.id}) in m'.clients // client ends up locked on this server
-    && Server(s.id, false) in m'.servers // server ends up locked
-    && (m.servers - {s}) == (m'.servers - {Server(s.id, false)}) // no other changes
-    && (m.clients - {c}) == (m'.clients - {Client(c.id, c.connServers + {s.id})}) // no other changes
+predicate ActionConnect(m: DafnyState, m': DafnyState) {
+    exists c: Client, s: Server ::
+
+        && RelationSemaphore(m, s) // in original state
+        && RelationLink(m', c, s)
+        && !RelationSemaphore(m', s)
+
+        // TODO: might need to ensure client/server is in m.clients/m.servers on left side of implication
+        && forall cf: Client, sf: Server :: (cf.id != c.id ==> RelationLink(m, cf, sf) == RelationLink(m', cf, sf))
+        
+        && forall sf: Server :: (sf.id != s.id ==> RelationSemaphore(m, sf) == RelationSemaphore(m', sf))
+
+
+        /*
+        && c in m.clients // client exists
+        && s in m.servers // server exists
+        && s.semaphore == true // server is unlocked to start
+        && Client(c.id, c.connServers + {s.id}) in m'.clients // client ends up locked on this server
+        && Server(s.id, false) in m'.servers // server ends up locked
+        && (m.servers - {s}) == (m'.servers - {Server(s.id, false)}) // no other changes
+        && (m.clients - {c}) == (m'.clients - {Client(c.id, c.connServers + {s.id})}) // no other changes
+        */
 }
 
 // action disconnect(x:client,y:server) = {
@@ -36,22 +78,41 @@ predicate Connect(m: DafnyStateMachine, m': DafnyStateMachine, c: Client, s: Ser
 //   link(x,y) := false;
 //   semaphore(y) := true
 // }
-predicate Disconnect(m: DafnyStateMachine, m': DafnyStateMachine, c: Client, s: Server) {
-    && c in m.clients // client exists
+predicate ActionDisconnect(m: DafnyState, m': DafnyState) {
+    exists c: Client, s: Server ::
+
+        && !RelationSemaphore(m, s) // in original state
+        && !RelationLink(m', c, s)
+        && RelationSemaphore(m', s)
+
+        && forall cf: Client, sf: Server :: (cf.id != c.id ==> RelationLink(m, cf, sf) == RelationLink(m', cf, sf))
+        
+        && forall sf: Server :: (sf.id != s.id ==> RelationSemaphore(m, sf) == RelationSemaphore(m', sf))
+
+   /* && c in m.clients // client exists
     && s in m.servers // server exists
     && s.id in c.connServers // client held server lock
     && Client(c.id, c.connServers - {s.id}) in m'.clients // client ends up unlocked on this server
     && Server(s.id, true) in m'.servers // server ends up unlocked
     && (m.servers - {s}) == (m'.servers - {Server(s.id, true)}) // no other changes
-    && (m.clients - {c}) == (m'.clients - {Client(c.id, c.connServers - {s.id})}) // no other changes
+    && (m.clients - {c}) == (m'.clients - {Client(c.id, c.connServers - {s.id})}) // no other changes*/
 }
 
-predicate Next(m:DafnyStateMachine, m':DafnyStateMachine) {
-    || (exists c:Client, s:Server :: Connect(m, m', c, s))
-    || (exists c:Client, s:Server :: Disconnect(m, m', c, s))
+predicate Next(m:DafnyState, m':DafnyState) {
+    //|| (exists c:Client, s:Server :: Connect(m, m', c, s))
+    //|| (exists c:Client, s:Server :: Disconnect(m, m', c, s))
+    || ActionConnect(m, m')
+    || ActionDisconnect(m, m')
 }
 
 // export connect
 // export disconnect
 
 // invariant [1000000] link(C1, S) & link(C2, S) -> C1 = C2
+lemma Invariant(m: DafnyState) 
+    ensures forall c1: Client, c2:Client, s: Server :: 
+    (c1 in m.clients && c2 in m.clients && s in m.servers) ==> (RelationLink(m, c1, s) && RelationLink(m, c2, s) ==> c1.id == c2.id)
+{
+    // somehow need to prove that safety property
+}
+
